updates

Veritas.Verifier.Merkle.fst
@@ -1,8 +1,66 @@
 module Veritas.Verifier.Merkle
 
+open FStar.Seq
+open Veritas.BinTree
 open Veritas.BinTreePtr
+
 open Veritas.EAC
+open Veritas.Interleave
+open Veritas.Key
+open Veritas.Record
 open Veritas.Verifier
 open Veritas.Verifier.CorrectDefs
 
-let eac_ptrfn (#n:nat) (itsl: its_log n): ptrfn = admit()
+
+(* eac_value is either empty or points to a a descendant *)
+let lemma_eac_value_empty_or_points_to_desc 
+  (#p:pos) 
+  (itsl: eac_ts_log p)
+  (k:key{is_merkle_key k})
+  (c:bin_tree_dir):
+  Lemma (requires True)
+        (ensures (mv_points_to_none (to_merkle_value (eac_value itsl k)) c \/ 
+                  is_desc (mv_pointed_key (to_merkle_value (eac_value itsl k)) c) (child c k)))
+  = admit()
+
+let eac_ptrfn_aux (#p:pos) (itsl: eac_ts_log p) (n:bin_tree_node) (c:bin_tree_dir):
+  option (d:bin_tree_node{is_desc d (child c n)}) = 
+  if depth n >= key_size then None
+  else
+    let v = to_merkle_value (eac_value itsl n) in
+    let dh = desc_hash_dir v c in
+    match dh with
+    | Empty -> None
+    | Desc dk _ _ -> 
+      lemma_eac_value_empty_or_points_to_desc itsl n c;
+      Some dk
+
+let eac_ptrfn (#p:pos) (itsl: eac_ts_log p): ptrfn =
+  eac_ptrfn_aux itsl
+
+let lemma_has_add_equiv_root_reachable 
+  (#p:pos) 
+  (itsl:eac_ts_log p) (k:merkle_key{k <> Root}):
+  Lemma (requires (True))
+        (ensures (has_some_add_of_key k (project_seq itsl) <==> root_reachable (eac_ptrfn itsl) k))
+  = admit()
+
+
+let proving_ancestor (#p:pos) (itsl: eac_ts_log p) (k:key{k <> Root}): 
+    k':key{is_proper_desc k k'} = admit()
+
+(* after the first add the proving ancestor always points to self *)
+let lemma_proving_ancestor_points_to_self (#p:pos) (itsl: eac_ts_log p) (k:key{k <> Root}):
+  Lemma (requires not (is_eac_state_init itsl k))
+        (ensures (mv_points_to (to_merkle_value (eac_value itsl (proving_ancestor itsl k)))
+                               (desc_dir k (proving_ancestor itsl k))
+                               k)) = admit()
+
+(* before the first add the proving ancestor points to none or to a key that is not an ancestor *)
+let lemma_proving_ancestor_initial (#p:pos) (itsl: eac_ts_log p) (k:key{k <> Root}):
+  Lemma (requires (is_eac_state_init itsl k))
+        (ensures (mv_points_to_none (to_merkle_value (eac_value itsl (proving_ancestor itsl k)))
+                                    (desc_dir k (proving_ancestor itsl k)) \/
+                  not (is_desc k (mv_pointed_key (to_merkle_value (eac_value itsl (proving_ancestor itsl k)))
+                                                 (desc_dir k (proving_ancestor itsl k)))))) = admit()
+
