Veritas.Verifier.Merkle.fsti
@@ -1,0 +1,37 @@
+module Veritas.Verifier.Merkle
+
+open Veritas.BinTree
+open Veritas.Key
+open Veritas.Record
+open Veritas.Verifier.CorrectDefs
+
+let mv_points_to_none (v: merkle_value) (d:bin_tree_dir): bool = 
+  desc_hash_dir v d = Empty
+
+let mv_points_to_some (v:merkle_value) (d:bin_tree_dir): bool = 
+  Desc? (desc_hash_dir v d) 
+
+let mv_pointed_key (v:merkle_value) (d:bin_tree_dir{mv_points_to_some v d}): key = 
+  Desc?.k (desc_hash_dir v d)
+
+let mv_points_to (v:merkle_value) (d:bin_tree_dir) (k:key): bool = 
+  mv_points_to_some v d && mv_pointed_key v d = k
+
+(* the ancestor who holds the proof of the value of key k *)
+val proving_ancestor (#p:pos) (itsl: eac_ts_log p) (k:key{k <> Root}):
+  k':key{is_proper_desc k k'}
+
+(* after the first add the proving ancestor always points to self *)
+val lemma_proving_ancestor_points_to_self (#p:pos) (itsl: eac_ts_log p) (k:key{k <> Root}):
+  Lemma (requires not (is_eac_state_init itsl k))
+        (ensures (mv_points_to (to_merkle_value (eac_value itsl (proving_ancestor itsl k)))
+                               (desc_dir k (proving_ancestor itsl k))
+                               k))
+
+(* before the first add the proving ancestor points to none or to a key that is not an ancestor *)
+val lemma_proving_ancestor_initial (#p:pos) (itsl: eac_ts_log p) (k:key{k <> Root}):
+  Lemma (requires (is_eac_state_init itsl k))
+        (ensures (mv_points_to_none (to_merkle_value (eac_value itsl (proving_ancestor itsl k)))
+                                    (desc_dir k (proving_ancestor itsl k)) \/
+                  not (is_desc k (mv_pointed_key (to_merkle_value (eac_value itsl (proving_ancestor itsl k)))
+                                                 (desc_dir k (proving_ancestor itsl k))))))
